The client of our "veric" Separation Logic will import only:
msl.standard
msl.normalize
veric.base
veric.expr
veric.seplog
veric.SeparationLogic*

this last one can be replace with, for example, an instance of SeparationLogic
such as SequentialClight.

The current commit cleans things up by removing from (base,expr,seplog)
all the things that the client should not see.  This required splitting
expr into two files, the "interface" (expr.v) and the "internals"
(expr_lemmas.v).

veric/seplog.v
@@ -87,9 +87,6 @@ Definition env_set (rho: environ) (x: ident) (v: val) : environ :=
 Definition subst (x: ident) (v: val) (P: assert) : assert :=
    fun s => P (env_set s x v).
 
-Definition val2adr' (v: val): address :=
- match v with Vptr b i => (b, Int.unsigned i) | _ => (0,0) end.
-
 Definition mapsto' (sh: Share.t) (e1: Clight.expr) (v2 : val): assert :=
  fun rho => 
   match access_mode (Clight.typeof e1) with
@@ -101,30 +98,6 @@ Definition mapsto' (sh: Share.t) (e1: Clight.expr) (v2 : val): assert :=
     end
   | _ => FF
   end. 
-
-Definition mapsto (sh: Share.t) (e1: Clight.expr) (e2 : Clight.expr) : assert :=
- fun rho =>  mapsto' sh e1 (eval_expr rho e2) rho.
-
-Definition expr_eq (e1 e2 : Clight.expr) : assert :=  
-   fun rho => !! (eval_expr rho e1 = eval_expr rho e2).
-
-Notation "e '==' f" := (expr_eq e f) (at level 25, no associativity): assert. 
-Notation "e1 '|->' e2" := (mapsto Share.top e1 AST.Mint32 e2) (at level 25, no associativity): assert.
-
-Definition exprlist_eq (e1 e2: list Clight.expr) : assert :=
-   fun rho =>  !! (map (eval_expr rho) e1 = map (eval_expr rho) e2).
-
-Definition assert_env := nat -> assert.
-Definition assert_env_nil : assert_env := fun n rho => FF.
-
-Definition assert_env_cons (hd: assert) (tl:  assert_env) (n: nat) : assert :=
-   match n with O => hd | S n' => tl n' end.
-
-Lemma f_assert_env_cons: forall f hd tl i,
-    f (assert_env_cons hd tl i) = assert_env_cons (f hd) (fun n => f (tl n)) i.
-Proof.
-induction i; auto.
-Qed.
 
 Definition writable_block (id: ident) (n: Z): assert :=
    fun rho => 
@@ -142,12 +115,12 @@ Definition fun_assert:
   forall  (v: val) (fml: funsig) (A: Type) (P Q: A -> list val -> pred rmap), pred rmap :=
   res_predicates.fun_assert.
 
-Inductive exitkind : Type := EK_normal | EK_break | EK_continue | EK_return.
-
-Definition ret_assert := exitkind -> list val -> assert.
-
 Definition lvalue_block (rsh: Share.t) (e: Clight.expr) : assert :=
-  fun rho => VALspec_range (sizeof (Clight.typeof e)) rsh Share.top (val2adr' (eval_lvalue rho e)).
+  fun rho => 
+     match eval_lvalue rho e with 
+     | Vptr b i => VALspec_range (sizeof (Clight.typeof e)) rsh Share.top (b, Int.unsigned i)
+     | _ => FF
+    end.
 
 Definition var_block (rsh: Share.t) (idt: ident * type) : assert :=
          lvalue_block rsh (Clight.Evar (fst idt) (snd idt)).
@@ -158,18 +131,6 @@ Fixpoint sepcon_list {A}{JA: Join A}{PA: Perm_alg A}{SA: Sep_alg A}{AG: ageable 
 
 Definition stackframe_of (f: Clight.function) : assert :=
   fun rho => sepcon_list (map (fun idt => var_block Share.top idt rho) (Clight.fn_vars f)).
-
-Instance EqDec_exitkind: EqDec exitkind.
-Proof.
-hnf. intros.
-decide equality.
-Qed.
-
-Definition overridePost  (Q: assert)  (R: ret_assert) := 
-     fun ek vl => if eq_dec ek EK_normal then (fun rho => !! (vl=nil) && Q rho) else R ek vl.
-
-Definition existential_ret_assert {A: Type} (R: A -> ret_assert) := 
-  fun ek vl rho => Ex x:A, R x ek vl rho.
 
 Lemma  subst_extens: 
  forall a v P Q, (forall rho, P rho |-- Q rho) -> forall rho, subst a v P rho |-- subst a v Q rho.
@@ -186,12 +147,6 @@ Inductive funspec :=
 
 Definition funspecs := list (ident * funspec).
 
-Fixpoint zip_arguments (vl: list val) (tl: typelist) : list (val * type) :=
-  match vl, tl with
-  | v::vl', Tcons t tl' => (v,t) :: zip_arguments vl' tl'
-  | _, _ => nil
- end.
-
 Definition bind_args (formals: list (ident * type)) (P: list val -> pred rmap) : assert :=
    fun rho => let vl := map (fun xt => (eval_expr rho (Etempvar (fst xt) (snd xt)))) formals
           in !! (typecheck_vals vl (map (@snd _ _) formals) = true) && P vl.
@@ -203,7 +158,7 @@ Definition bind_ret (vl: list val) (t: type) (Q: list val -> pred rmap) : pred r
      | _, _ => FF
      end.
 
-Definition func (f: funspec): address -> pred rmap :=
+Definition func_at (f: funspec): address -> pred rmap :=
   match f with
    | mk_funspec fsig A P Q => pureat (SomeP (A::boolT::(list val)::nil) (packPQ P Q)) (FUN fsig)
   end.
@@ -216,9 +171,9 @@ Definition funassert (G: funspecs) : assert :=
    (All  id: ident, All fs:funspec,  !! In (id,fs) G -->
               Ex v:val, Ex loc:address, 
                    !! (ge_of rho id = Some (v, type_of_funspec fs)
-                                 /\ val2adr v loc) && func fs loc)
+                                 /\ val2adr v loc) && func_at fs loc)
    && 
-   (All  loc: address, All fs:funspec, func fs loc --> 
+   (All  loc: address, All fs:funspec, func_at fs loc --> 
              Ex id:ident,Ex v:val,  !! (ge_of rho id = Some (v, type_of_funspec fs)
                                  /\ val2adr v loc) && !! In (id,fs) G).
 
@@ -249,22 +204,6 @@ Lemma address_mapsto_VALspec_range:
        |-- VALspec_range (size_chunk ch) rsh sh l.
 Proof.  exact address_mapsto_VALspec_range. Qed.
 
-
-Definition normal_ret_assert (Q: assert) : ret_assert := 
-   fun ek vl rho => !!(ek = EK_normal) && (!! (vl = nil) && Q rho).
-
-Definition with_ge (ge: genviron) (G: assert) : pred rmap :=
-     G (mkEnviron ge (Maps.PTree.empty _) (Maps.PTree.empty _)).
-
-Lemma resource_at_identity: forall (m: rmap) (loc: address), 
- identity m -> identity (m @ loc).
-Proof.
-  intros.
-  destruct (@resource_at_empty m H loc) as [?|[? [? ?]]].
-  rewrite H0. apply NO_identity.
-  rewrite H0. apply PURE_identity.
-Qed.
-
 Lemma VALspec_range_0: forall rsh sh loc, VALspec_range 0 rsh sh loc = emp.
   Proof.
    intros.
@@ -279,6 +218,7 @@ Lemma VALspec_range_0: forall rsh sh loc, VALspec_range 0 rsh sh loc = emp.
    do 3 red. apply resource_at_identity; auto.
    destruct loc, b; intros [? ?]; simpl in *; omega.
 Qed.
+Hint Resolve VALspec_range_0: normalize.
 
 Lemma VALspec_range_split2:
   forall (n m r: Z) (rsh sh: Share.t) (b: block) (ofs: Z),
@@ -343,6 +283,29 @@ generalize (Address.size_chunk_pos ch2); intro;
 destruct a2; split; auto; omega.
 auto.
 Qed.
+
+
+Inductive exitkind : Type := EK_normal | EK_break | EK_continue | EK_return.
+
+Instance EqDec_exitkind: EqDec exitkind.
+Proof.
+hnf. intros.
+decide equality.
+Qed.
+
+Definition ret_assert := exitkind -> list val -> assert.
+
+Definition overridePost  (Q: assert)  (R: ret_assert) := 
+     fun ek vl => if eq_dec ek EK_normal then (fun rho => !! (vl=nil) && Q rho) else R ek vl.
+
+Definition existential_ret_assert {A: Type} (R: A -> ret_assert) := 
+  fun ek vl rho => Ex x:A, R x ek vl rho.
+
+Definition normal_ret_assert (Q: assert) : ret_assert := 
+   fun ek vl rho => !!(ek = EK_normal) && (!! (vl = nil) && Q rho).
+
+Definition with_ge (ge: genviron) (G: assert) : pred rmap :=
+     G (mkEnviron ge (Maps.PTree.empty _) (Maps.PTree.empty _)).
 
 Definition frame_ret_assert (R: ret_assert) (F: assert) : ret_assert := 
       fun ek vl rho => R ek vl rho * F rho.
