veric/base.v
@@ -22,15 +22,6 @@ Definition genviron := ident -> option (val*type).
 Inductive environ : Type :=
  mkEnviron: forall (ge: genviron) (ve: Clight.env) (te: Clight.temp_env), environ.
 
-Definition filter_genv (ge: Clight.genv) : genviron :=
-  fun id => match Genv.find_symbol ge id with
-                   | Some b => match Clight.type_of_global ge b with
-                                        | Some t => Some (Vptr b Int.zero, t)
-                                        | None => Some (Vptr b Int.zero, Tvoid)
-                                        end
-                   | None => None
-                   end. 
-
 Definition ge_of (rho: environ) : genviron :=
   match rho with mkEnviron ge ve te => ge end.
 
@@ -39,11 +30,6 @@ Definition ve_of (rho: environ) : Clight.env :=
 
 Definition te_of (rho: environ) : Clight.temp_env :=
   match rho with mkEnviron ge ve te => te end.
-
-Definition mkEnviron' (ge: Clight.genv) (ve: Clight.env) (te: Clight.temp_env) :=
-  mkEnviron (filter_genv ge) ve te.
-
-Definition empty_environ (ge: Clight.genv) := mkEnviron (filter_genv ge) (Maps.PTree.empty _) (Maps.PTree.empty _).
 
 Definition opt2list (A: Type) (x: option A) :=
   match x with Some a => a::nil | None => nil end.
@@ -56,4 +42,40 @@ Fixpoint typelist2list (tl: typelist) : list type :=
  match tl with Tcons t r => t::typelist2list r | Tnil => nil end.
 
 Definition funsig := (typelist * type)%type. (* argument and result signature *)
+
+Definition modified0 : ident -> Prop := fun _ => False.
+Definition modified1 id : ident -> Prop := fun i => i=id.
+Definition modified2 (s1 s2: ident -> Prop) := fun i => s1 i \/ s2 i.
+
+Fixpoint modifiedvars (c: statement) : ident -> Prop :=
+ match c with
+ | Sset id e => modified1 id
+ | Sifthenelse _ c1 c2 => modified2 (modifiedvars c1) (modifiedvars c2)
+ | Scall (Some id) _ _ => modified1 id
+ | Ssequence c1 c2 =>  modified2 (modifiedvars c1) (modifiedvars c2)
+ | Swhile e c => modifiedvars c
+ | Sdowhile e c => modifiedvars c
+ | Sfor' e c1 c2 => modified2 (modifiedvars c1) (modifiedvars c2)
+ | Sswitch e cs => modifiedvars_ls cs
+ | Slabel _ c => modifiedvars c
+ | _ => modified0
+ end
+ with
+ modifiedvars_ls (cs: labeled_statements) : ident -> Prop := 
+ match cs with
+ | LSdefault _ => modified0
+ | LScase _ c ls => modified2 (modifiedvars c) (modifiedvars_ls ls)
+ end.
+
+
+Definition filter_genv (ge: Clight.genv) : genviron :=
+  fun id => match Genv.find_symbol ge id with
+                   | Some b => match Clight.type_of_global ge b with
+                                        | Some t => Some (Vptr b Int.zero, t)
+                                        | None => Some (Vptr b Int.zero, Tvoid)
+                                        end
+                   | None => None
+                   end. 
+
+Definition empty_environ (ge: Clight.genv) := mkEnviron (filter_genv ge) (Maps.PTree.empty _) (Maps.PTree.empty _).
 
