veric/expr_lemmas.v
@@ -1,0 +1,412 @@
+Require Import msl.msl_standard.
+Require Import veric.base.
+Require Import veric.Address.
+Require Import msl.rmaps.
+Require Import msl.rmaps_lemmas.
+Require Import veric.compcert_rmaps.
+Require Import veric.Clight_lemmas.
+Require Import veric.expr.
+
+Definition mkEnviron' (ge: Clight.genv) (ve: Clight.env) (te: Clight.temp_env) :=
+  mkEnviron (filter_genv ge) ve te.
+
+Definition Delta1 : tycontext := (PTree.set 1%positive (type_int32s, false) (PTree.empty (type * bool)),
+                                 PTree.empty type, Tvoid).
+
+
+Definition temp_element_correct (te : temp_env) :=
+(fun (tyconEl : (PTree.elt * type)) => let (id,elt) := tyconEl in
+  match te ! id with
+  | Some v => typecheck_val v elt = true
+  | _ => False
+end). 
+
+Definition te_correct (te : temp_env) (Delta: tycontext) := Forall
+  (temp_element_correct te)
+  (map remove_assignedness (PTree.elements (temp_types Delta))).
+
+Definition var_element_correct (ve: env) (ge:genviron) : 
+(PTree.elt * type) -> Prop :=
+(fun (varel : (PTree.elt * type)) => let (id,ty) := varel in
+  match ve ! id with
+  | Some (_,ty') => if type_eq ty ty' then True else False
+  | None => match (ge id) with
+        | Some (v,ty2') => if type_eq ty ty2' && 
+                              typecheck_val v ty2' &&
+                              is_pointer_type ty2'(*Double check===================================*)
+                              (*^will be correct with change to base.v*)
+        then True else False 
+        | None => False
+        end
+  end).
+
+Definition ve_correct (ve:env) (ge:genviron) (Delta: tycontext) :=
+Forall (var_element_correct ve ge) (PTree.elements (var_types Delta)).
+
+
+Lemma typecheck_environ_sound : forall ge te ve Delta,
+typecheck_environ (mkEnviron ge ve te) Delta = true ->
+te_correct te Delta /\ ve_correct ve ge Delta.
+Proof.
+intros.
+unfold typecheck_environ in *. destruct Delta. destruct p.
+unfold te_correct. unfold ve_correct.
+unfold temp_types in *. simpl in *. split.
+
+induction (PTree.elements t0).
+constructor. 
+unfold temp_element_correct.
+simpl in *. destruct a. destruct p0. rewrite Forall_forall; intros.
+destruct x. simpl in *. destruct H0. inv H0. destruct (te!e). 
+destruct (typecheck_val v t3). auto. inv H. inv H.
+destruct (te!p). remember (typecheck_val v t2) as b0. destruct b0. 
+intuition. rewrite Forall_forall in *. unfold temp_element_correct in *.
+specialize (H1 (e,t3)). intuition. inv H. inv H.
+
+unfold var_types in *; simpl in *. rewrite andb_true_iff in H. destruct H.
+clear H. rewrite Forall_forall. intros. 
+destruct x. induction (PTree.elements t1). inv H.
+simpl in *. destruct a. destruct H. inv H. destruct (ve !e). destruct p.
+destruct (type_eq t2 t3). auto. inv H0. destruct (ge e). destruct p.
+destruct (type_eq t2 t3 && typecheck_val v t3 && is_pointer_type t3). auto.
+intuition. inv H0. 
+apply IHl.
+clear IHl.  destruct (ve ! p). destruct p0. 
+destruct (type_eq t3 t4). subst.
+auto. inv H0. destruct (ge p). destruct p0. 
+destruct (type_eq t3 t4 && typecheck_val v t4 && is_pointer_type t4).
+auto. inv H0. inv H0. auto. 
+Qed.
+
+Lemma typecheck_te_sound : forall dv te,
+typecheck_temp_environ dv te = true ->
+Forall (temp_element_correct te) dv.
+Proof.
+intros. induction dv. auto.
+simpl in *. destruct a. remember (te! p). destruct o; auto.
+remember (typecheck_val v t) as b0. destruct b0. 
+rewrite Forall_forall. intros. simpl in H0. destruct H0. inv H0.
+unfold temp_element_correct. rewrite <- Heqo. auto. intuition.
+rewrite Forall_forall in H1. apply H1. auto. inv H. inv H.
+Qed.
+
+Lemma in_fst_in : forall A B (L : list (A*B)) (a:A) (b:B), In (a, b) L  -> In a (map (@fst A B) L) .
+Proof.
+intros A B L. induction L; intros. auto. simpl in *. inv H. auto. right. eapply IHL. apply H0.
+Qed.
+
+Lemma in_rem_in : forall A B C (L : list (A*(B*C))) a b c,
+In (a, (b, c)) L -> In (a,b) (map remove_assignedness (L)).
+intros A B C L. induction L; intros. inv H. simpl in *.
+inv H. left. auto. right. eapply  IHL. eauto.
+Qed.
+
+(*I think I need this eventually
+but can't figure it out right now...
+Lemma typecheck_environ_put_te : forall ge te ve Delta id v ,
+typecheck_environ (mkEnviron ge ve te) Delta = true ->
+(*((temp_types Delta) ! id = Some t ->
+  (typecheck_val v (fst t)) = true) ->*)
+(*typecheck_expr Delta (Etempvar id (typeof e)) = true ->
+typecheck_expr Delta e = true ->*) 
+typecheck_environ (mkEnviron ge ve (PTree.set id v te)) Delta = true.
+Proof.
+intros. unfold typecheck_environ in *. simpl in *. repeat rewrite andb_true_iff in *.
+intuition. clear H1. destruct Delta. destruct p. unfold temp_types in *; simpl in *.
+
+remember (map remove_assignedness (PTree.elements t0)).
+generalize dependent t0.
+induction l; intros; auto.
+
+simpl in *. destruct  a.  
+remember (te ! p). destruct o; intuition.
+remember (typecheck_val v0 t2). destruct b0; intuition.
+remember ((PTree.set id v te) ! p).
+destruct o. remember (typecheck_val v1 t2). destruct b0.
+eapply H.
+Focus 2. clear H.
+assert (typecheck_val v1 t2 = true). 
+apply typecheck_te_sound in H0. rewrite Forall_forall in *.
+unfold temp_element_correct in H0.
+clear Heqb1. 
+
+Focus 3. clear H.   
+assert (In (p,t3) (p,t3::l)).
+assert (x:=eq_dec p id). destruct x. subst. rewrite PTree.gss in Heqo0.
+inv Heqo0. apply typecheck_te_sound in H1. rewrite Forall_forall in H1.
+unfold temp_element_correct in H1.
+
+unfold typecheck_temp_environ in H. 
+ rewrite typecheck_environ_sound in H1. 
+*)
+
+
+
+Lemma no_rep_in_pair : forall A B L a b b2, list_norepet (map (@fst A B) (L)) ->
+  In (a, b) L -> In (a,b2) L -> b = b2.
+Proof.
+intros A B L. induction L; intros. inv H0. simpl in *.
+inv H. intuition.
+  destruct a. inv H0. inv H. auto.
+ 
+  destruct H4. destruct a; simpl. inv H. eapply in_fst_in. eauto. 
+  
+  destruct H4. destruct a; simpl. inv H0. eapply in_fst_in. eauto.
+
+  eapply IHL; eauto.
+Qed. 
+
+
+Lemma type_eq_true : forall a b, proj_sumbool  (type_eq a b) =true  -> a = b.
+Proof. intros. destruct (type_eq a b). auto. simpl in H. inv H.
+Qed.
+
+Ltac of_bool_destruct :=
+match goal with
+  | [ |- context[Val.of_bool ?X] ] => destruct X
+end.
+
+
+Lemma classify_add_int_cases_both : forall i1 s1 a1 i2 s2 a2,
+exists s3,
+classify_add (Tint i1 s1 a1) (Tint i2 s2 a2) 
+= add_case_ii s3.
+Proof.
+intros; destruct i1; destruct s1; destruct i2; destruct s2; eexists;  
+unfold classify_add; simpl; eauto.
+Qed.
+
+Lemma undef_not_typecheck : forall t, typecheck_val Vundef t = false.
+intros.
+destruct t; auto.
+Qed.
+
+
+
+(*come back here
+Lemma typecheck_binop_sound:
+forall (Delta : tycontext) (rho : environ) (b0 : binary_operation)
+  (e1 e2 : expr) (t : type),
+typecheck_expr Delta e2 = true ->
+isBinOpResultType b0 e1 e2 t = true ->
+typecheck_expr Delta e1 = true ->
+typecheck_val (eval_expr rho e2) (typeof e2) = true ->
+typecheck_val (eval_expr rho e1) (typeof e1) = true ->
+typecheck_val (eval_expr rho (Ebinop b0 e1 e2 t)) t = true.
+Proof.
+Admitted. (*for memory, proof below should work*)
+(*intros.
+unfold eval_expr in *. simpl in *.
+destruct b0; simpl in *;
+match goal with 
+| [ |- typecheck_val ( force_val (?X _ _ _ _)) _ = true ] => unfold X in *
+| [ |- typecheck_val ( force_val (?X _ _ _ _ _)) _ = true ] => unfold X in *
+| [ |- typecheck_val ( force_val (?X _ _ _ _ _ _)) _ = true ] => unfold X in *
+end;(
+do 2
+(match goal with
+| [ |- context[(typeof ?X)]] => let x := fresh "tofx" in remember (typeof X) as x; destruct x
+end); intuition; simpl;
+try solve [try destruct i; try destruct s; try destruct i0; try destruct s0; intuition;(
+simpl in *;
+try solve [do 2 try
+match goal with
+| [ |- context[compute_expr ?ge ?ve ?te ?e]] => remember (compute_expr ge ve te e) as compR; destruct compR
+end; try destruct t; auto; intuition; try (of_bool_destruct; auto)])]). 
+Qed.*) *)
+
+Lemma typecheck_both_sound: 
+  forall Delta rho e P, 
+             typecheck_environ rho Delta = true -> 
+             (typecheck_expr Delta e = P ->
+              denote_tc_assert P rho ->
+             typecheck_val (eval_expr rho e) (typeof e) = true) /\
+             (forall pt, typecheck_lvalue Delta e = P -> 
+             denote_tc_assert P rho ->
+             is_pointer_type pt = true -> 
+             typecheck_val (eval_lvalue rho e) pt=true).
+Proof.
+intros. induction e; intuition.
+Admitted. (*So I can get it committed
+(*Const int*)
+simpl. destruct t; auto; simpl in H0; inv H0; intuition.
+
+(*Const float*)
+simpl in *. destruct t; intuition. 
+
+(*Var*)
+simpl in *. unfold eval_lvalue. simpl.
+
+apply typecheck_environ_sound in H. destruct H.
+clear H. unfold ve_correct in H2. rewrite Forall_forall in *.
+unfold var_element_correct in *.
+remember ((var_types Delta) ! i). destruct o; intuition. rewrite andb_true_iff in *.
+intuition. apply type_eq_true in H. subst. symmetry in Heqo.
+apply PTree.elements_correct in Heqo.
+specialize (H2 (i,t0)). intuition.
+remember ((ve_of rho) ! i). destruct o.
+destruct p. remember (type_eq t0 t). destruct s; intuition.
+subst. rewrite H3. destruct pt; auto.
+destruct (ge_of rho i); auto. destruct p. 
+remember (@proj_sumbool (t0 = t) (t0 = t -> False) (type_eq t0 t) &&
+       typecheck_val v t && is_pointer_type t).
+destruct b0; try contradiction. symmetry in Heqb0. repeat rewrite andb_true_iff in *. intuition.
+destruct (type_eq t0 t); auto. subst. admit.
+(*Stuck. If an int can typecheck as a pointer, should it be able to
+check as struct and union in the same cases??*)
+ (* Focus 2. destruct v; 
+destruct t; auto; intuition. destruct pt; intuition. 
+
+
+simpl in *. simpl in H5. simpl in *. simpl in *.
+ destruct t; auto.
+destruct t; auto.
+auto.*)
+
+(*Temp*)
+simpl in *. destruct rho. apply typecheck_environ_sound in H. intuition. 
+unfold te_correct in *. unfold temp_element_correct in *.
+rewrite Forall_forall in *. clear H2. 
+
+unfold eval_expr. unfold compute_expr. simpl. unfold force_val.
+destruct Delta. destruct p. 
+unfold temp_types in *. simpl in *.
+remember (t1 ! i). destruct o.
+  symmetry in Heqo. apply PTree.elements_correct in Heqo. 
+  destruct p. specialize (H1 (i,t3)). simpl in H1.
+apply type_eq_true in H0. inv H0. simpl in *.
+apply in_rem_in in Heqo. intuition. destruct (te ! i); auto.
+inv H0.  
+
+(*deref  -- no proof now, doesn't typecheck
+simpl in *. rewrite andb_true_iff in *; intuition. 
+unfold eval_lvalue. simpl. unfold eval_expr in *.
+remember (compute_expr (ge_of rho) (ve_of rho) (te_of rho) e).
+destruct v; intuition; destruct (typeof e); intuition. simpl in *. 
+*)
+
+(*addrof*)
+unfold eval_expr in *. simpl in *. rewrite andb_true_iff in *; intuition. 
+destruct t. Focus 4. simpl in *. apply H2. unfold typecheck_lvalue_pure in *.a
+
+(*Unop*)
+simpl in *. rewrite andb_true_iff in *. intuition.
+unfold eval_expr in *; destruct u; simpl in *. 
+
+unfold sem_notbool in *.
+remember (typeof e). destruct t0; simpl in *; intuition; try destruct i; try destruct s; simpl in *;
+destruct ((compute_expr (ge_of rho) (ve_of rho) (te_of rho) e)); intuition;
+simpl; try of_bool_destruct; try destruct t; intuition.
+
+unfold sem_notint. remember (typeof e). destruct t0; simpl in *; 
+try destruct i; try destruct s; intuition;
+destruct (compute_expr (ge_of rho) (ve_of rho) (te_of rho) e);
+simpl in *; try of_bool_destruct; destruct t; intuition.
+
+unfold sem_neg. remember (typeof e). destruct t0; simpl in *; 
+try destruct i; try destruct s; intuition;
+destruct (compute_expr (ge_of rho) (ve_of rho) (te_of rho) e);
+simpl in *; try of_bool_destruct; destruct t; intuition.
+
+(*binop*)
+simpl in *. repeat rewrite andb_true_iff in *; intuition.
+clear H1. clear H3. clear H.
+
+eapply typecheck_binop_sound; eauto.
+
+(* cast *)
+simpl. unfold eval_expr. simpl. simpl in *. rewrite andb_true_iff in *; intuition.
+unfold eval_expr in *. remember (compute_expr (ge_of rho) (ve_of rho) (te_of rho) e).
+destruct v; intuition; remember (typeof e); destruct t0; intuition; destruct t; intuition;
+try destruct i; try destruct i0; try destruct i1; intuition.
+
+(*condition*)
+simpl in *. repeat rewrite andb_true_iff in *; intuition.
+unfold eval_expr in *.
+simpl in *. 
+remember (compute_expr (ge_of rho) (ve_of rho) (te_of rho) e2).
+remember (compute_expr (ge_of rho) (ve_of rho) (te_of rho) e3).
+
+destruct ((compute_expr (ge_of rho) (ve_of rho) (te_of rho) e1)); intuition.
+remember (typeof e1); destruct t0; intuition. simpl.
+destruct (negb (Int.eq i Int.zero)). destruct v; intuition; remember (typeof e2);
+destruct t0; intuition; destruct t; intuition; try destruct i2; try destruct s0; intuition;
+try destruct i3; try destruct s0; try destruct s1; try destruct i1; intuition.
+destruct v0; intuition; remember (typeof e3); destruct t0; intuition; destruct t; intuition; 
+try destruct i2; try destruct s0; intuition;
+try destruct i3; try destruct s0; try destruct s1; try destruct i1; intuition.
+remember (typeof e1); destruct t0; intuition. simpl.
+destruct (negb (Float.cmp Ceq f Float.zero)).
+remember (typeof e2). destruct v; destruct t0; destruct t; intuition;
+try destruct i0; try destruct s; intuition; try destruct i1; try destruct s0; try destruct i; intuition.
+remember (typeof e3). destruct v0; destruct t0; destruct t; intuition; 
+try destruct i0; try destruct s; intuition; try destruct i1; try destruct s0; try destruct i; intuition.
+remember (typeof e1). unfold bool_val. destruct t0; intuition.
+
+(*EField*)
+simpl in H2. rewrite andb_true_iff in *; intuition. unfold eval_lvalue in *.
+unfold eval_expr in *.
+simpl.
+remember (compute_expr (ge_of rho) (ve_of rho) (te_of rho) e).
+destruct v; intuition; 
+remember (typeof e); destruct t0; intuition. 
+
+remember (field_offset i f). destruct r; intuition.
+
+Qed. *)
+
+Lemma typecheck_expr_sound : forall Delta rho e P,
+ typecheck_environ rho Delta = true -> 
+             (typecheck_expr Delta e = P ->
+              denote_tc_assert P rho ->
+             typecheck_val (eval_expr rho e) (typeof e) = true).
+Proof. intros. 
+assert (TC := typecheck_both_sound Delta rho e P). intuition. Qed.
+
+
+(*Figure out where this is used, would not hold when pointers typecheck as
+ints*)
+Lemma get_typed_int:
+    forall v att, typecheck_val v (Tint I32 Signed att) = true -> 
+                      exists i:int, v = Vint i.
+intros; destruct v; inv H; eauto.
+Qed.
+
+Definition is_ptr_type (ty: type) : bool :=
+  match ty with
+  | Tpointer _ _ => true
+  | Tarray _ _ _ => true
+  | Tfunction _ _ => true
+  | Tstruct _ _ _ => true
+  | Tunion _ _ _ => true
+  | _ => false
+end.
+
+(*Not going to work because of null pointer
+Lemma get_typed_ptr:
+   forall v ty, 
+                   typecheck_val v ty = true -> 
+                   is_ptr_type ty = true ->
+                      exists b, exists ofs, v = Vptr b ofs.
+Proof.
+intros; destruct v; destruct ty; inv H; eauto; inv H0.
+Qed.*)
+
+
+Lemma eval_expr_relate:
+  forall Delta ge rho e m,
+              filter_genv ge = ge_of rho ->
+              typecheck_environ rho Delta = true ->
+              tc_expr Delta e rho ->
+              Clight_sem.eval_expr ge (ve_of rho) (te_of rho) m e  (eval_expr rho e).
+Admitted.
+
+Lemma eval_lvalue_relate:
+  forall Delta ge rho e m,
+              filter_genv ge = ge_of rho ->
+              typecheck_environ rho Delta = true ->
+              tc_lvalue Delta e rho ->
+              exists b, exists ofs, 
+              Clight_sem.eval_lvalue ge (ve_of rho) (te_of rho) m e b ofs /\
+              eval_lvalue rho e = Vptr b ofs.
+Admitted. 
