veric/semax.v
@@ -14,7 +14,7 @@ Require Import veric.Clight_lemmas.
 Require Import veric.extspec.
 Require Import veric.step_lemmas.
 Require Import veric.juicy_extspec.
-Require Import veric.expr.
+Require Import veric.expr veric.expr_lemmas.
 
 Local Open Scope nat_scope.
 Local Open Scope pred.
